src/ldrfra/RARace.v
@@ -30,7 +30,7 @@ Require Import JoinedView.
 Require Import LocalDRFPFView.
 
 Require Import OrdStep.
-Require Import Stable.
+Require Import Writes.
 Require Import WStep.
 Require Import PFtoRA.
 
@@ -41,11 +41,30 @@ Module RARace.
 Section RARACE.
   Variable L: Loc.t -> bool.
 
+  Definition wr_race (loc: Loc.t) (to: Time.t) (ordw: Ordering.t) (tview: TView.t) (ord: Ordering.t): Prop :=
+    (<<LOC: L loc>>) /\
+    (<<HIGHER: Time.lt ((View.rlx (TView.cur tview)) loc) to>>) /\
+    ((<<ORDW: Ordering.le ordw Ordering.strong_relaxed>>) \/
+     (<<ORDR: Ordering.le ord Ordering.strong_relaxed>>)).
+
+  Definition ww_race (loc: Loc.t) (to: Time.t) (ordw: Ordering.t) (tview: TView.t) (ord: Ordering.t): Prop :=
+    (<<LOC: L loc>>) /\
+    (<<HIGHER: Time.lt ((View.rlx (TView.cur tview)) loc) to>>) /\
+    ((<<ORDW1: Ordering.le ordw Ordering.na>>) \/
+     (<<ORDW2: Ordering.le ord Ordering.na>>)).
+
+  Definition ra_race (loc: Loc.t) (to: Time.t) (ordw: Ordering.t) (tview: TView.t) (e: ProgramEvent.t): Prop :=
+    (exists loc val ord,
+        (<<READ: ProgramEvent.is_reading e = Some (loc, val, ord)>>) /\
+        (<<WRRACE: wr_race loc to ordw tview ord>>)) \/
+    (exists loc val ord,
+        (<<WRITE: ProgramEvent.is_writing e = Some (loc, val, ord)>>) /\
+        (<<WWRACE: ww_race loc to ordw tview ord>>)).
+
   Definition race (c1: Configuration.t): Prop :=
     exists c2 c3
-           tid_w e_w loc from to val released ordw
-           tid_r lang st3 lc3 e4 e5
-           pf e_r released' ordr,
+      tid_w e_w loc from to val released ordw
+      tid_r lang st3 lc3 e4 e st5,
       (<<WRITE_STEP: OrdConfiguration.step L Ordering.acqrel Ordering.acqrel e_w tid_w c1 c2>>) /\
       (<<WRITE_EVENT: ThreadEvent.is_writing e_w = Some (loc, from, to, val, released, ordw)>>) /\
       (<<STEPS2: rtc (@OrdConfiguration.all_step L Ordering.acqrel Ordering.acqrel) c2 c3>>) /\
@@ -54,20 +73,144 @@ Section RARACE.
                            (Thread.mk _ st3 lc3 (Configuration.sc c3) (Configuration.memory c3))
                            e4>>) /\
       (<<CONS: Local.promise_consistent (Thread.local e4)>>) /\
-      (<<READ_STEP: OrdThread.step L Ordering.acqrel Ordering.acqrel pf e_r e4 e5>>) /\
-      (<<READ_EVENT: ThreadEvent.is_reading e_r = Some (loc, to, val, released', ordr)>>) /\
-      (<<LOC: L loc>>) /\
-      (<<HIGHER: Time.lt ((Local.tview (Thread.local e4)).(TView.cur).(View.rlx) loc) to>>) /\
-      (<<ORDERING: __guard__(Ordering.le ordw Ordering.strong_relaxed \/
-                             Ordering.le ordr Ordering.strong_relaxed)>>).
+      (<<STEP: lang.(Language.step) e e4.(Thread.state) st5>>) /\
+      (<<RACE: ra_race loc to ordw (Local.tview (Thread.local e4)) e>>).
 
   Definition racefree (c: Configuration.t): Prop :=
-    forall c1
-           (STEPS1: rtc (@OrdConfiguration.all_step L Ordering.acqrel Ordering.acqrel) c c1),
+    forall c1 (STEPS1: rtc (@OrdConfiguration.all_step L Ordering.acqrel Ordering.acqrel) c c1),
       ~ race c1.
 
   Definition racefree_syn (s: Threads.syntax): Prop :=
     racefree (Configuration.init s).
 
+
+  Lemma read_message_exists
+        lang
+        rels1 rels2 e1 e2
+        loc to ordw
+        (PROMISES: OrdLocal.reserve_only L (Local.promises (Thread.local e1)))
+        (WF1: Local.wf (Thread.local e1) (Thread.memory e1))
+        (SC1: Memory.closed_timemap (Thread.sc e1) (Thread.memory e1))
+        (MEM1: Memory.closed (Thread.memory e1))
+        (STEPS: @WThread.steps lang L Ordering.acqrel Ordering.acqrel rels1 rels2 e1 e2)
+        (RELS2: List.In (loc, to, ordw) rels2)
+        (HIGHER: Time.lt ((Local.tview (Thread.local e2)).(TView.cur).(View.rlx) loc) to):
+    (<<RELS1: List.In (loc, to, ordw) rels1>>).
+  Proof.
+    dependent induction STEPS; try by (esplits; eauto).
+    hexploit WThread.step_reserve_only; try exact STEP; eauto. i. des.
+    exploit WThread.step_future; eauto. i. des.
+    exploit WThread.steps_future; try exact STEPS; eauto. i. des.
+    exploit IHSTEPS; eauto. i. des.
+    clear IHSTEPS. revert x.
+    inv STEP. inv STEP0; inv STEP; [|inv LOCAL]; ss; try by (esplits; eauto).
+    - unfold Writes.append. ss. condtac; ss. i. des; ss. inv x.
+      assert (Time.le to ((TView.cur (Local.tview lc2)).(View.rlx) loc)).
+      { inv LOCAL0. inv STEP. ss.
+        unfold TimeMap.join, TimeMap.singleton.
+        unfold LocFun.add, LocFun.init, LocFun.find. condtac; ss.
+        apply Time.join_r.
+      }
+      inv TVIEW_FUTURE0. inv CUR. rewrite (RLX loc) in H0. timetac.
+    - unfold Writes.append. ss. condtac; ss. i. des; ss. inv x.
+      assert (Time.le to ((TView.cur (Local.tview lc2)).(View.rlx) loc)).
+      { inv LOCAL2. inv STEP. ss.
+        unfold TimeMap.join, TimeMap.singleton.
+        unfold LocFun.add, LocFun.init, LocFun.find. condtac; ss.
+        apply Time.join_r.
+      }
+      inv TVIEW_FUTURE0. inv CUR. rewrite (RLX loc) in H0. timetac.
+    - unfold Writes.append. ss. condtac; ss. i. des; ss. inv x.
+      assert (Time.le to ((TView.cur (Local.tview lc2)).(View.rlx) loc)).
+      { inv LOCAL0.
+        - inv STEP. ss.
+          unfold TimeMap.join, TimeMap.singleton.
+          unfold LocFun.add, LocFun.init, LocFun.find. condtac; ss.
+          apply Time.join_r.
+        - inv STEP. ss.
+          unfold TimeMap.join, TimeMap.singleton.
+          unfold LocFun.add, LocFun.init, LocFun.find. condtac; ss.
+          apply Time.join_r.
+      }
+      inv TVIEW_FUTURE0. inv CUR. rewrite (RLX loc) in H0. timetac.
+  Qed.
+
+  Lemma write_exists
+        ordr ordw
+        rels1 rels2 c1 c2
+        loc to ord
+        (WF1: Configuration.wf c1)
+        (STEPS: WConfiguration.steps L ordr ordw rels1 rels2 c1 c2)
+        (LOC: L loc)
+        (RELS1: ~ List.In (loc, to, ord) rels1)
+        (RELS2: List.In (loc, to, ord) rels2):
+    exists rels11 rels12 c11 c12 tid e from val released,
+      (<<STEPS1: WConfiguration.steps L ordr ordw rels1 rels11 c1 c11>>) /\
+      (<<WRITE_STEP: WConfiguration.step L ordr ordw e tid rels11 rels12 c11 c12>>) /\
+      (<<WRITE_EVENT: ThreadEvent.is_writing e = Some (loc, from, to, val, released, ord)>>) /\
+      (<<STEPS2: WConfiguration.steps L ordr ordw rels12 rels2 c12 c2>>).
+  Proof.
+    revert WF1. induction STEPS; i; try congr.
+    exploit WConfiguration.step_future; eauto. i. des.
+    exploit WConfiguration.step_rels; eauto. i. subst.
+    destruct (classic (exists from val released,
+                          ThreadEvent.is_writing e = Some (loc, from, to, val, released, ord))).
+    { des. esplits; eauto. econs 1. }
+    exploit IHSTEPS; eauto.
+    { unfold Writes.append. des_ifs. ii. ss. des; ss. inv H0. eauto. }
+    i. des. esplits; eauto. econs 2; eauto.
+  Qed.
+
+  Lemma racefree_implies
+        s
+        (RACEFREE: racefree_syn s):
+    RARaceW.racefree_syn L Ordering.acqrel Ordering.acqrel s.
+  Proof.
+    specialize (@Configuration.init_wf s). intro WF.
+    specialize (@OrdConfiguration.init_reserve_only L s). intro RESERVE.
+    ii. unfold RARaceW.ra_race in *. des.
+    { destruct WRRACE as [to [ordw [LOC [HIGHER [IN ORD]]]]]. guardH ORD. des.
+      unfold racefree_syn in *.
+      remember (Configuration.init s) as c1. clear Heqc1.
+      exploit WConfiguration.steps_future; eauto. intro WF2. des.
+      hexploit OrdConfiguration.rtc_all_step_reserve_only;
+        try eapply WConfiguration.steps_ord_steps; eauto. intro RESERVE2.
+      dup WF2. inv WF0. inv WF1. exploit THREADS; eauto. i.
+      clear DISJOINT THREADS.
+      unfold OrdConfiguration.reserve_only in RESERVE2.
+      hexploit RESERVE2; eauto. i.
+      hexploit read_message_exists; try exact THREAD_STEPS; eauto. i. des.
+      exploit write_exists; try exact STEPS; eauto. i. des.
+      exploit WConfiguration.steps_ord_steps; try exact STEPS1. i.
+      exploit WConfiguration.step_ord_step; try exact WRITE_STEP. i.
+      exploit WConfiguration.steps_ord_steps; try exact STEPS2. i.
+      exploit WThread.steps_ord_steps; eauto. i.
+      eapply RACEFREE; eauto.
+      unfold race. esplits; eauto.
+      left. esplits; eauto.
+      unfold wr_race. splits; auto.
+    }
+    { destruct WWRACE as [to [ordw [LOC [HIGHER [IN ORD]]]]]. guardH ORD. des.
+      unfold racefree_syn in *.
+      remember (Configuration.init s) as c1. clear Heqc1.
+      exploit WConfiguration.steps_future; eauto. intro WF2. des.
+      hexploit OrdConfiguration.rtc_all_step_reserve_only;
+        try eapply WConfiguration.steps_ord_steps; eauto. intro RESERVE2.
+      dup WF2. inv WF0. inv WF1. exploit THREADS; eauto. i.
+      clear DISJOINT THREADS.
+      unfold OrdConfiguration.reserve_only in RESERVE2.
+      hexploit RESERVE2; eauto. i.
+      hexploit read_message_exists; try exact THREAD_STEPS; eauto. i. des.
+      exploit write_exists; try exact STEPS; eauto. i. des.
+      exploit WConfiguration.steps_ord_steps; try exact STEPS1. i.
+      exploit WConfiguration.step_ord_step; try exact WRITE_STEP. i.
+      exploit WConfiguration.steps_ord_steps; try exact STEPS2. i.
+      exploit WThread.steps_ord_steps; eauto. i.
+      eapply RACEFREE; eauto.
+      unfold race. esplits; eauto.
+      right. esplits; eauto.
+      unfold ww_race. splits; auto.
+    }
+  Qed.
 End RARACE.
 End RARace.
